add thms

Barrel/Builtins/Arithmetic.lean
@@ -1,28 +1,29 @@
 import Barrel.Builtins.Init
 import Barrel.Builtins.Power
 import Barrel.Builtins.Function
+import Barrel.Builtins.Relation
 import Mathlib.Data.Set.Basic
+import Mathlib.Data.Set.Finite.Basic
 import Mathlib.Data.Fintype.Lattice
 import Mathlib.Data.Fintype.EquivFin
 import Mathlib.Data.Int.Interval
 import Mathlib.Order.Interval.Finset.Defs
-
 namespace B.Builtins
   open Classical
 
   abbrev interval (lo hi : ℤ) : Set Int := Set.Icc lo hi
   scoped infixl:170 ".." => interval
 
-  structure min.WF {α : Type _} [LinearOrder α] (S : Set α) : Prop where
+  structure min.WF {α : Type _} [PartialOrder α] (S : Set α) : Prop where
     isBoundedBelow : ∃ x ∈ S, ∀ y ∈ S, x ≤ y
 
-  noncomputable abbrev min {α : Type _} [LinearOrder α] (S : Set α) (wf : min.WF S) : α :=
+  noncomputable abbrev min {α : Type _} [PartialOrder α] (S : Set α) (wf : min.WF S) : α :=
     Classical.choose wf.isBoundedBelow
 
-  structure max.WF {α : Type _} [LinearOrder α] (S : Set α) : Prop where
+  structure max.WF {α : Type _} [PartialOrder α] (S : Set α) : Prop where
     isBoundedAbove : ∃ x ∈ S, ∀ y ∈ S, y ≤ x
 
-  noncomputable abbrev max {α : Type _} [LinearOrder α] (S : Set α) (wf : max.WF S) : α :=
+  noncomputable abbrev max {α : Type _} [PartialOrder α] (S : Set α) (wf : max.WF S) : α :=
     Classical.choose wf.isBoundedAbove
 
   structure card.WF {α : Type _} (S : Set α) : Prop where
@@ -179,6 +180,60 @@ namespace B.Builtins
       exists lo
       and_intros <;> grind
 
+    @[grind →]
+    theorem min.mem {α : Type _} [PartialOrder α] {S : Set α} (wf : min.WF S) :
+        min S wf ∈ S := (Classical.choose_spec wf.isBoundedBelow).1
+
+    @[grind →]
+    theorem max.mem {α : Type _} [PartialOrder α] {S : Set α} (wf : max.WF S) :
+        max S wf ∈ S := (Classical.choose_spec wf.isBoundedAbove).1
+
+    @[grind .]
+    theorem min.WF_of_union {α : Type _} [LinearOrder α] {S T : Set α}
+        (hS : min.WF S) (hT : min.WF T) : min.WF (S ∪ T) := by
+      obtain ⟨s_min, s_min_mem, s_min_bnd⟩ := hS
+      obtain ⟨t_min, t_min_mem, t_min_bnd⟩ := hT
+      let m := if s_min ≤ t_min then s_min else t_min
+      exists m
+      and_intros
+      · unfold m
+        split_ifs with hm
+        · exact Set.mem_union_left T s_min_mem
+        · exact Set.mem_union_right S t_min_mem
+      · rintro y (hy | hy)
+        · unfold m
+          split_ifs with hm
+          · exact s_min_bnd y hy
+          · exact le_trans (le_of_not_ge hm) (s_min_bnd y hy)
+        · unfold m
+          split_ifs with hm
+          · exact le_trans hm (t_min_bnd y hy)
+          · exact t_min_bnd y hy
+
+    @[grind .]
+    theorem max.WF_of_union {α : Type _} [LinearOrder α] {S T : Set α}
+        (hS : max.WF S) (hT : max.WF T) : max.WF (S ∪ T) := by
+      obtain ⟨s_max, s_max_mem, s_max_bnd⟩ := hS
+      obtain ⟨t_max, t_max_mem, t_max_bnd⟩ := hT
+      let m := if t_max ≤ s_max then s_max else t_max
+      exists m
+      and_intros
+      · unfold m
+        split_ifs with hm
+        · exact Set.mem_union_left T s_max_mem
+        · exact Set.mem_union_right S t_max_mem
+      · rintro y (hy | hy)
+        · unfold m
+          split_ifs with hm
+          · exact s_max_bnd y hy
+          · exact le_trans
+              (le_trans (s_max_bnd y hy) (le_of_not_ge hm))
+              (t_max_bnd t_max t_max_mem)
+        · unfold m
+          split_ifs with hm
+          · exact le_trans (t_max_bnd y hy) hm
+          · exact t_max_bnd y hy
+
     @[grind ., simp]
     theorem interval.min_eq {lo hi : Int} (h : lo ≤ hi) :
         min (lo .. hi) (min.WF_interval h) = lo := by
@@ -195,28 +250,140 @@ namespace B.Builtins
       obtain ⟨m_def, m_is_max⟩ := Classical.choose_spec hm
       exact le_antisymm m_def.2 (m_is_max _ (Set.right_mem_Icc.mpr h))
 
-    theorem min.WF_singleton {α : Type _} [LinearOrder α] {a : α} : min.WF {a} :=
-      min.WF_of_finite <| FIN₁.singleton_mem (Set.mem_singleton a)
+    theorem min.WF_singleton {α : Type _} [PartialOrder α] {a : α} : min.WF {a} :=
+      ⟨a, Set.mem_singleton a, fun _ ↦ ge_of_eq⟩
 
-    theorem max.WF_singleton {α : Type _} [LinearOrder α] {a : α} : max.WF {a} :=
-      max.WF_of_finite <| FIN₁.singleton_mem (Set.mem_singleton a)
+    theorem max.WF_singleton {α : Type _} [PartialOrder α] {a : α} : max.WF {a} :=
+      ⟨a, Set.mem_singleton a, fun _ ↦ le_of_eq⟩
 
     @[simp]
-    theorem min.of_singleton {α : Type _} [LinearOrder α] {a : α} :
+    theorem min.of_singleton {α : Type _} [PartialOrder α] {a : α} :
         min {a} (min.WF_singleton) = a := by
       unfold min
       generalize_proofs ha
       exact (Classical.choose_spec ha).1
 
+    @[grind .]
+    theorem min.WF_of_insert {α : Type _} [LinearOrder α] {S : Set α} (a : α)
+        (hS : min.WF S) : min.WF (insert a S) := by
+      obtain ⟨s_min, s_min_mem, s_min_bnd⟩ := hS
+      let m := if a ≤ s_min then a else s_min
+      exists m
+      unfold m
+      split_ifs with hm
+      · and_intros
+        · exact Set.mem_insert a S
+        · intro y hy
+          rw [Set.mem_insert_iff] at hy
+          obtain rfl | hy := hy
+          · exact le_refl y
+          · exact le_trans hm (s_min_bnd y hy)
+      · and_intros
+        · exact Set.mem_insert_of_mem a s_min_mem
+        · intro y hy
+          rw [Set.mem_insert_iff] at hy
+          obtain rfl | hy := hy
+          · exact le_of_not_ge hm
+          · exact s_min_bnd y hy
+
+    @[grind ., simp]
+    theorem min.of_insert {α : Type _} [LinearOrder α] {S : Set α} (a : α)
+        (hS : min.WF S) :
+        min (insert a S) (min.WF_of_insert a hS) =
+          if a ≤ min S hS then a else min S hS := by
+      unfold min
+      split_ifs with ha
+      · generalize_proofs h₁ h₂ at ha ⊢
+        obtain ⟨m_def, m_is_min⟩ := Classical.choose_spec h₂
+        obtain ⟨s_min_def, s_min_is_min⟩ := Classical.choose_spec h₁
+        set m := choose h₂
+        set s_min := choose h₁
+        rw [Set.mem_insert_iff] at m_def
+        obtain m_eq | m_in := m_def
+        · exact m_eq
+        · apply le_antisymm
+            (m_is_min _ (Set.mem_insert a S))
+            (le_trans ha (s_min_is_min m m_in))
+      · generalize_proofs h₁ h₂
+        obtain ⟨m_def, m_is_min⟩ := Classical.choose_spec h₂
+        obtain ⟨s_min_def, s_min_is_min⟩ := Classical.choose_spec h₁
+        set m := choose h₂
+        set s_min := choose h₁
+        rw [Set.mem_insert_iff] at s_min_def
+        obtain s_min_eq | s_min_in := s_min_def
+        · rw [←s_min_eq] at ha
+          rw [not_le] at ha
+          simp at s_min_is_min
+          nomatch lt_irrefl _ (lt_of_le_of_lt (s_min_is_min.2 m m_def) ha)
+        · apply le_antisymm
+            (s_min_is_min _ (Set.mem_insert_of_mem a m_def))
+            (m_is_min s_min s_min_in)
+
+    @[grind .]
+    theorem max.WF_of_insert {α : Type _} [LinearOrder α] {S : Set α} (a : α)
+        (hS : max.WF S) : max.WF (insert a S) := by
+      obtain ⟨s_max, s_max_mem, s_max_bnd⟩ := hS
+      let m := if s_max ≤ a then a else s_max
+      exists m
+      unfold m
+      split_ifs with hm
+      · and_intros
+        · exact Set.mem_insert a S
+        · intro y hy
+          rw [Set.mem_insert_iff] at hy
+          obtain rfl | hy := hy
+          · exact le_refl y
+          · exact le_trans (s_max_bnd y hy) hm
+      · and_intros
+        · exact Set.mem_insert_of_mem a s_max_mem
+        · intro y hy
+          rw [Set.mem_insert_iff] at hy
+          obtain rfl | hy := hy
+          · exact le_of_not_ge hm
+          · exact s_max_bnd y hy
+
+    @[grind ., simp]
+    theorem max.of_insert {α : Type _} [LinearOrder α] {S : Set α} (a : α)
+        (hS : max.WF S) :
+        max (insert a S) (max.WF_of_insert a hS) =
+          if max S hS ≤ a then a else max S hS := by
+      unfold max
+      split_ifs with ha
+      · generalize_proofs h₁ h₂ at ha ⊢
+        obtain ⟨m_def, m_is_max⟩ := Classical.choose_spec h₂
+        obtain ⟨s_max_def, s_max_is_max⟩ := Classical.choose_spec h₁
+        set m := choose h₂
+        set s_max := choose h₁
+        rw [Set.mem_insert_iff] at m_def
+        obtain m_eq | m_in := m_def
+        · exact m_eq
+        · apply le_antisymm
+            (le_trans (s_max_is_max m m_in) ha)
+            (m_is_max _ (Set.mem_insert a S))
+      · generalize_proofs h₁ h₂
+        obtain ⟨m_def, m_is_max⟩ := Classical.choose_spec h₂
+        obtain ⟨s_max_def, s_max_is_max⟩ := Classical.choose_spec h₁
+        set m := choose h₂
+        set s_max := choose h₁
+        rw [Set.mem_insert_iff] at s_max_def
+        obtain s_max_eq | s_max_in := s_max_def
+        · rw [←s_max_eq] at ha
+          rw [not_le] at ha
+          simp at s_max_is_max
+          nomatch lt_irrefl _ (lt_of_le_of_lt (s_max_is_max.2 m m_def) ha)
+        · apply le_antisymm
+            (m_is_max s_max s_max_in)
+            (s_max_is_max _ (Set.mem_insert_of_mem a m_def))
+
     @[simp]
-    theorem max.of_singleton {α : Type _} [LinearOrder α] {a : α} :
+    theorem max.of_singleton {α : Type _} [PartialOrder α] {a : α} :
         max {a} (max.WF_singleton) = a := by
       unfold max
       generalize_proofs ha
       exact (Classical.choose_spec ha).1
 
     @[grind .]
-    theorem max.ge_min {α : Type _} [LinearOrder α] {S : Set α}
+    theorem max.ge_min {α : Type _} [PartialOrder α] {S : Set α}
         (hmax : max.WF S) (hmin : min.WF S) :
         max S hmax ≥ min S hmin := by
       unfold max min
@@ -226,9 +393,123 @@ namespace B.Builtins
       exact is_max (choose hmin) min_def
 
     @[grind .]
-    theorem min.le_max {α : Type _} [LinearOrder α] {S : Set α}
+    theorem min.le_max {α : Type _} [PartialOrder α] {S : Set α}
       (hmin : min.WF S) (hmax : max.WF S) :
         min S hmin ≤ max S hmax := max.ge_min hmax hmin
+
+    theorem min.WF_of_finite_image_pfun {α β : Type _} [LinearOrder β] {A : Set α } {B : Set β}
+      {f : SetRel α β} {S : Set α} (hf : f ∈ A ⇸ B) (hS : S ∈ FIN₁ (dom f)) :
+        min.WF (f[S]) := by
+      apply min.WF_of_finite (A := f[S])
+      and_intros
+      · exact subset_refl _
+      · obtain ⟨⟨Sdom, Sfin⟩, Snemp⟩ := hS
+        let S' := Set.Finite.toFinset Sfin
+        suffices f[S'].Finite by
+          apply Set.Finite.subset this
+          intro x hx
+          obtain ⟨w, wS, wxf⟩ := hx
+          exists w, ?_
+          · simpa [S']
+          · exact wxf
+        induction S' using Finset.induction with
+        | empty => simp only [Finset.coe_empty, SetRel.image_empty_right, Set.finite_empty]
+        | insert x S notMem IH =>
+          have : f[insert x S] = f[{x}] ∪ f[S] := by ext; simp
+          simp only [Finset.coe_insert, this, Set.finite_union]
+          and_intros
+          · by_cases hx : x ∈ dom f
+            · obtain ⟨y, hy⟩ := hx
+              have : f[{x}] = {y} := by
+                ext z
+                simp only [SetRel.image, Set.mem_singleton_iff, exists_eq_left, Set.mem_setOf_eq]
+                constructor
+                · exact (hf.2 · hy)
+                · rintro rfl
+                  exact hy
+              rw [this]
+              exact Set.finite_singleton y
+            · have : f[{x}] = ∅ := by
+                ext z
+                simp only [SetRel.image, Set.mem_singleton_iff, exists_eq_left, Set.mem_setOf_eq,
+                  Set.mem_empty_iff_false, iff_false]
+                exact fun contr ↦ nomatch hx ⟨z, contr⟩
+              rw [this]
+              exact Set.finite_empty
+          · exact IH
+      · obtain ⟨⟨sub_dom, _⟩, s, hs⟩ := hS
+        obtain ⟨w, hw⟩ := sub_dom hs
+        exists w, s
+
+    theorem min.WF_of_finite_image_tfun {α β : Type _} [LinearOrder β] {A : Set α } {B : Set β}
+      {f : SetRel α β} {S : Set α} (hf : f ∈ A ⟶ B) (hS : S ∈ FIN₁ A) :
+        min.WF (f[S]) := by
+      apply min.WF_of_finite_image_pfun (Set.mem_of_mem_inter_left hf)
+      rwa [tfun_dom_eq hf]
+
+    theorem max.WF_of_finite_image_pfun {α β : Type _} [LinearOrder β] {A : Set α } {B : Set β}
+      {f : SetRel α β} {S : Set α} (hf : f ∈ A ⇸ B) (hS : S ∈ FIN₁ (dom f)) :
+        max.WF (f[S]) := by
+      apply max.WF_of_finite (A := f[S])
+      and_intros
+      · exact subset_refl _
+      · obtain ⟨⟨Sdom, Sfin⟩, Snemp⟩ := hS
+        let S' := Set.Finite.toFinset Sfin
+        suffices f[S'].Finite by
+          apply Set.Finite.subset this
+          intro x hx
+          obtain ⟨w, wS, wxf⟩ := hx
+          exists w, ?_
+          · simpa [S']
+          · exact wxf
+        induction S' using Finset.induction with
+        | empty => simp only [Finset.coe_empty, SetRel.image_empty_right, Set.finite_empty]
+        | insert x S notMem IH =>
+          have : f[insert x S] = f[{x}] ∪ f[S] := by ext; simp
+          simp only [Finset.coe_insert, this, Set.finite_union]
+          and_intros
+          · by_cases hx : x ∈ dom f
+            · obtain ⟨y, hy⟩ := hx
+              have : f[{x}] = {y} := by
+                ext z
+                simp only [SetRel.image, Set.mem_singleton_iff, exists_eq_left, Set.mem_setOf_eq]
+                constructor
+                · exact (hf.2 · hy)
+                · rintro rfl
+                  exact hy
+              rw [this]
+              exact Set.finite_singleton y
+            · have : f[{x}] = ∅ := by
+                ext z
+                simp only [SetRel.image, Set.mem_singleton_iff, exists_eq_left, Set.mem_setOf_eq,
+                  Set.mem_empty_iff_false, iff_false]
+                exact fun contr ↦ nomatch hx ⟨z, contr⟩
+              rw [this]
+              exact Set.finite_empty
+          · exact IH
+      · obtain ⟨⟨sub_dom, _⟩, s, hs⟩ := hS
+        obtain ⟨w, hw⟩ := sub_dom hs
+        exists w, s
+
+    theorem max.WF_of_finite_image_tfun {α β : Type _} [LinearOrder β] {A : Set α } {B : Set β}
+      {f : SetRel α β} {S : Set α} (hf : f ∈ A ⟶ B) (hS : S ∈ FIN₁ A) :
+        max.WF (f[S]) := by
+      apply max.WF_of_finite_image_pfun (Set.mem_of_mem_inter_left hf)
+      rwa [tfun_dom_eq hf]
+
+    @[grind .]
+    theorem min.mono {α : Type _} [PartialOrder α] {S T : Set α} (hsub : T ⊆ S)
+      (hS : min.WF S) (hT : min.WF T) : min S hS ≤ min T hT :=
+        (choose_spec hS.isBoundedBelow).right
+          (choose hT.isBoundedBelow)
+          (hsub (choose_spec hT.isBoundedBelow).left)
+
+    @[grind .]
+    theorem max.mono {α : Type _} [PartialOrder α] {S T : Set α} (hsub : S ⊆ T)
+      (hS : max.WF S) (hT : max.WF T) : max S hS ≤ max T hT :=
+        (choose_spec hT.isBoundedAbove).right
+          (choose hS.isBoundedAbove)
+          (hsub (choose_spec hS.isBoundedAbove).left)
 
     @[grind ., simp]
     theorem card.WF_of_empty {α : Type _} : card.WF (∅ : Set α) where
@@ -257,7 +538,6 @@ namespace B.Builtins
       · rw [Int.sub_nonneg]
         exact Int.le_add_one h
 
-
     @[grind .]
     theorem card.WF_of_subset {α : Type _} {S T : Set α} (hS : S ⊆ T)
         (hT : card.WF T) : card.WF S where
@@ -271,6 +551,15 @@ namespace B.Builtins
         card.WF S where
       isFinite := h.1.2
 
+    @[grind .]
+    theorem card.WF_of_singleton {α : Type _} {a : α} : card.WF {a} where
+      isFinite := Set.finite_singleton a
+
+    @[simp]
+    theorem card.of_singleton {α : Type _} {a : α} :
+        card {a} WF_of_singleton = 1 := by
+      simp only [card, Set.toFinset_singleton, Finset.card_singleton, Nat.cast_one]
+
     @[grind →]
     theorem card.mono {α : Type _} {S T : Set α} (hS : S ⊆ T) (hT : card.WF T) :
         card S (card.WF_of_subset hS hT) ≤ card T hT := by
@@ -279,6 +568,73 @@ namespace B.Builtins
       have : Finite ↑S := (card.WF_of_subset hS hT).isFinite
       have : Finite ↑T := hT.isFinite
       exact @Set.toFinset_mono α S T (Fintype.ofFinite ↑S) (Fintype.ofFinite ↑T) hS
+
+    @[grind .]
+    theorem card.WF_of_inter {α : Type _} {S T : Set α} (h : card.WF S ∨ card.WF T) :
+        card.WF (S ∩ T) where
+      isFinite := by
+        rcases h with hS | hT
+        · exact Set.Finite.inter_of_left hS.isFinite _
+        · exact Set.Finite.inter_of_right hT.isFinite _
+
+    @[grind .]
+    theorem card.WF_of_union {α : Type _} {S T : Set α} (hS : card.WF S) (hT : card.WF T) :
+        card.WF (S ∪ T) where
+      isFinite := Set.Finite.union hS.isFinite hT.isFinite
+
+    @[grind .]
+    theorem card.WF_of_insert {α : Type _} {S : Set α} (a : α)
+        (hS : card.WF S) : card.WF (insert a S) where
+      isFinite := Set.Finite.insert a hS.isFinite
+
+    @[grind .]
+    theorem card.WF_of_insert' {α : Type _} {S : Set α} (a : α)
+        (hS : card.WF S) : card.WF (S ∪ {a}) where
+      isFinite := by simpa only [Set.union_singleton, Set.finite_insert] using hS.isFinite
+
+    @[grind ., simp]
+    theorem card.of_insert {α : Type _} {S : Set α} (a : α)  (hS : card.WF S) :
+        card (insert a S) (card.WF_of_insert a hS) =
+          if a ∈ S then card S hS else card S hS + 1 := by
+      split_ifs with ha
+      · conv =>
+          enter [1,1]
+          rw [Set.insert_eq_of_mem ha]
+      · unfold card
+        extract_lets h₁ h₂
+        simp only [Set.toFinset_insert, Set.toFinset_card]
+        rw [Finset.card_insert_eq_ite, ite_cond_eq_false _ _ (eq_false ?_)]
+        · simp only [Set.toFinset_card, Nat.cast_add, Nat.cast_one]
+        · rwa [Set.mem_toFinset]
+
+    @[grind .]
+    theorem card.WF_of_sdiff {α : Type _} {S T : Set α} (hS : card.WF S) : card.WF (S \ T) where
+      isFinite := Set.Finite.diff hS.isFinite
+
+    @[simp]
+    theorem card.of_sdiff {α : Type _} {S T : Set α} (hS : card.WF S) :
+        card (S \ T) (card.WF_of_sdiff hS) =
+          card S hS - card (S ∩ T) (WF_of_inter (Or.inl hS)) := by
+      admit
+
+    @[simp]
+    theorem card.of_diff_singleton {α : Type _} {S : Set α} (a : α) (hS : card.WF S) :
+        card (S \ {a}) (card.WF_of_sdiff hS) =
+          if a ∈ S then card S hS - 1 else card S hS := by
+      rw [card.of_sdiff hS]
+      split_ifs with ha
+      · have : S ∩ {a} = {a} := by
+          ext
+          simp
+          rintro rfl
+          assumption
+        simp only [this, of_singleton]
+      · have : S ∩ {a} = ∅ := by
+          ext
+          simp
+          rintro _ rfl
+          contradiction
+        simp only [this, of_empty, sub_zero]
 
   end Lemmas
 end B.Builtins
