Barrel/Builtins.lean
@@ -3,25 +3,35 @@ import Barrel.Builtins.Function
 import Barrel.Builtins.Power
 import Barrel.Builtins.Arithmetic
 
-  /-
-  TODO: add remaining Unicode characters
+section Lemmas
+open B.Builtins
 
-  `/<<:` ≔ `⊄`
-  `/<:` ≔ `⊈`
-  `/:` ≔ `∉`
-  `<=>` ≔ `⇔`
-  `/=` ≔ `≠`
-  `<=` ≔ `≤`
-  `>=` ≔ `≥`
-  `<<:` ≔ `⊂`
-  `<:` ≔ `⊆`
-  `{}` ≔ `∅`
-  `\` ≔ `∖`
-  `**` ≔ `×`
-  `<+` ≔ `` (missing)
-  `><` ≔ `⊗`
-  `||` ≔ `∥`
-  `~` ≔ `∼`
-  `:=` ≔ `≔`
+@[grind =, simp]
+theorem SetRel.image_insert {α β : Type _} (f : SetRel α β) (a : α) (S : Set α) :
+    f[insert a S] = f[{a}] ∪ f[S] := by ext; simp
 
-  -/
+end Lemmas
+
+
+/-
+TODO: add remaining Unicode characters
+
+`/<<:` ≔ `⊄`
+`/<:` ≔ `⊈`
+`/:` ≔ `∉`
+`<=>` ≔ `⇔`
+`/=` ≔ `≠`
+`<=` ≔ `≤`
+`>=` ≔ `≥`
+`<<:` ≔ `⊂`
+`<:` ≔ `⊆`
+`{}` ≔ `∅`
+`\` ≔ `∖`
+`**` ≔ `×`
+`<+` ≔ `` (missing)
+`><` ≔ `⊗`
+`||` ≔ `∥`
+`~` ≔ `∼`
+`:=` ≔ `≔`
+
+-/
